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so the joint entropy is given by
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= 1.81 bits (6.8)

Clearly the marginal probabilities are uniform: p(X = 1) = p(X = 0) = p(Y = 0) = p(Y =
1) = 0.5, so H (X) = H (Y ) = 1. Hence H (X,Y ) = 1.81 bits < H (X) + H (Y ) = 2 bits. In
fact, this upper bound on the joint entropy holds in general. If X and Y are independent, then
H (X,Y ) = H (X) + H (Y ), so the bound is tight. This makes intuitive sense: when the parts are
correlated in some way, it reduces the “degrees of freedom” of the system, and hence reduces the
overall entropy.

What is the lower bound on H (X,Y )? If Y is a deterministic function of X, then H (X,Y ) = H (X).
So

H (X,Y ) ≥ max{H (X) ,H (Y )} ≥ 0 (6.9)

Intuitively this says combining variables together does not make the entropy go down: you cannot
reduce uncertainty merely by adding more unknowns to the problem, you need to observe some data,
a topic we discuss in Sec. 6.1.4.

We can extend the definition of joint entropy from two variables to n in the obvious way.

6.1.4 Conditional entropy

The conditional entropy of Y given X is the uncertainty we have in Y after seeing X, averaged
over possible values for X:

H (Y |X) , Ep(X) [H (p(Y |X))] (6.10)

=
∑

x

p(x)H (p(Y |X = x)) = −
∑

x

p(x)
∑

y

p(y|x) log p(y|x) (6.11)

= −
∑

x,y

p(x, y) log p(y|x) = −
∑

x,y

p(x, y) log
p(x, y)

p(x)
(6.12)

= −
∑

x,y

p(x, y) log p(x, y) +
∑

x

p(x) log
1

p(x)
(6.13)

= H (X,Y )−H (X) (6.14)

If Y is a deterministic function of X, then knowing X completely determines Y , so H (Y |X) = 0.
If X and Y are independent, knowing X tells us nothing about Y and H (Y |X) = H (Y ). Since
H (X,Y ) ≤ H (Y ) + H (X), we have

H (Y |X) ≤ H (Y ) (6.15)
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160 Chapter 6. Information theory

6.2.2 Interpretation

We can rewrite the KL as follows:

KL (p‖q) =
K∑

k=1

pk log pk

︸ ︷︷ ︸
−H(p)

−
K∑

k=1

pk log qk

︸ ︷︷ ︸
H(p,q)

(6.30)

We recognize the first term as the negative entropy, and the second term as the cross entropy. Thus
we can interpret the KL divergence as the “extra number of bits” you need to pay when compressing
data samples from p using the incorrect distribution q as the basis of your coding scheme.

There are various other interpretations of KL divergence. See the sequel to this book, [Mur22], for
more information.

6.2.3 Example: KL divergence between two Gaussians

For example, one can show that the KL divergence between two multivariate Gaussian distributions
is given by

KL (N (x|µ1,Σ1)‖N (x|µ2,Σ2))

=
1

2

[
tr(Σ−1

2 Σ1) + (µ2 − µ1)>Σ−1
2 (µ2 − µ1)−D + log

(
det(Σ2)

det(Σ1)

)]
(6.31)

In the scalar case, this becomes

KL (N (x|µ1, σ1)‖N (x|µ2, σ2)) = log
σ2

σ1
+
σ2

1 + (µ1 − µ2)2

2σ2
2

− 1

2
(6.32)

6.2.4 Non-negativity of KL

In this section, we prove that the KL divergence is always non-negative.

Theorem 6.2.1. (Information inequality) KL (p‖q) ≥ 0 with equality iff p = q.

Proof. We now prove the theorem following [CT06, p28]. Let A = {x : p(x) > 0} be the support of
p(x). Using the convexity of the log function and Jensen’s inequality (Sec. B.4.3), we have that

−KL (p‖q) = −
∑

x∈A
p(x) log

p(x)

q(x)
=
∑

x∈A
p(x) log

q(x)

p(x)
(6.33)

≤ log
∑

x∈A
p(x)

q(x)

p(x)
= log

∑

x∈A
q(x) (6.34)

≤ log
∑

x∈X
q(x) = log 1 = 0 (6.35)

Since log(x) is a strictly concave function (− log(x) is convex), we have equality in Eq. (6.34) iff
p(x) = cq(x) for some c that tracks the fraction of the whole space X contained in A. We have
equality in Eq. (6.35) iff

∑
x∈A q(x) =

∑
x∈X q(x) = 1, which implies c = 1. Hence KL (p‖q) = 0 iff

p(x) = q(x) for all x.
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6.3. Mutual information 165

6.3.4 Conditional mutual information

We can define the conditional mutual information in the obvious way

I (X;Y |Z) , Ep(Z) [I(X;Y )|Z] (6.53)

= Ep(x,y,z)
[
log

p(x, y|z)
p(x|z)p(y|z)

]
(6.54)

= H (X|Z) + H (Y |Z)−H (X,Y |Z) (6.55)
= H (X|Z)−H (X|Y,Z) = H (Y |Z)−H (Y |X,Z) (6.56)
= H (X,Z) + H (Y,Z)−H (Z)−H (X,Y, Z) (6.57)
= I(Y ;X,Z)− I(Y ;Z) (6.58)

The last equation tells us that the conditional MI is the extra (residual) information that X tells us
about Y , excluding what we already knew about Y given Z alone.

We can rewrite Eq. (6.58) as follows:

I(Z, Y ;X) = I(Z;X) + I(Y ;X|Z) (6.59)

Generalizing to N variables, we get the chain rule for mutual information:

I (Z1, . . . , ZN ;X) =
N∑

n=1

I (Zn;X|Z1, . . . , Zn−1) (6.60)

6.3.5 Normalized mutual information

For some applications, it is useful to have a normalized measure of dependence, between 0 and 1. We
now discuss one way to construct such a measure.

First, note that

I (X;Y ) = H (X)−H (X|Y ) ≤ H (X) (6.61)
= H (Y )−H (Y |X) ≤ H (Y ) (6.62)

so

0 ≤ I (X;Y ) ≤ min (H (X) ,H (Y )) (6.63)

Therefore we can define the normalized mutual information as follows:

NMI(X,Y ) =
I (X;Y )

min (H (X) ,H (Y ))
≤ 1 (6.64)

This normalized mutual information ranges from 0 to 1. When NMI(X,Y ) = 0, I (X;Y ) = 0 so X
and Y are independent. Without loss of generality assume X has the higher entropy: NMI(X,Y ) =
1 =⇒ I (X;Y ) = H (X)−H (X|Y ) = H (X) =⇒ H (X|Y ) = 0 and so X is a deterministic function
of Y .
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6.3. Mutual information 169

An example of a sufficient statistic is the data itself, s(D) = D, but this is not very useful, since
it doesn’t summarize the data at all. Hence we define a minimal sufficient statistic s(D) as one
which is sufficient, and which contains no extra information about θ; thus s(D) maximally compresses
the data D without losing information which is relevant to predicting θ. More formally, we say s is a
minimal sufficient statistic for D if for all sufficient statistics s′(D) there is some function f such that
s(D) = f(s′(D)). We can summarize the situation as follows:

θ → s(D)→ s′(D)→ D (6.78)

Here s′(D) takes s(D) and adds redundant information to it, thus creating a one-to-many mapping.
For example, a minimal sufficient statistic for a set of N Bernoulli trials is simply N and N1 =∑
n I (Xn = 1), i.e., the number of successes. In other words, we don’t need to keep track of the

entire sequence of heads and tails and their ordering, we only need to keep track of the total number
of heads and tails. Similarlt, for inferring the mean of a Gaussian distribution with known variance
we only need to know the empirical mean and number of samples.

6.3.9 Fano’s inequality

A common method for feature selection is to pick input features Xd which have high mutual
information with the response variable Y . Below we justify why this is a reasonable thing to do.
In particular, we state a result, known as Fano’s inequality, which bounds the probability of
misclassification (for any method) in terms of the mutual information between the features X and
the class label Y .

Theorem 6.3.2. (Fano’s inequality) Consider an estimator Ŷ = f(X) such that Y → X → Ŷ forms
a Markov chain. Let E be the event Ŷ 6= Y , indicating that an error occured, and let Pe = P (Y 6= Ŷ )
be the probability of error. Then we have

H (Y |X) ≤ H
(
Y |Ŷ

)
≤ H (E) + Pe log |Y| (6.79)

Since H (E) ≤ 1, as we saw in Fig. 6.1, we can weaken this result to get

1 + Pe log |Y| ≥ H (Y |X) (6.80)

and hence

Pe ≥
H (Y |X)− 1

log |Y| (6.81)

Thus minimizing H (Y |X) (which can be done by maximizing I(X;Y )) will also minimize the lower
bound on Pe.

Proof. (From [CT06, p38].) Using the chain rule for entropy, we have

H
(
E, Y |Ŷ

)
= H

(
Y |Ŷ

)
+ H

(
E|Y, Ŷ

)

︸ ︷︷ ︸
=0

(6.82)

= H
(
E|Ŷ

)
+ H

(
Y |E, Ŷ

)
(6.83)
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